{$\vx = \bmx{c}2\\4\\-1\emx$, $\vy = \bmx{c} -1\\-3\\-1\emx$}
{$\vx+\vy = \bmx{c}1\\1\\-2\emx$, $\vx-\vy = \bmx{c} 3\\7\\0\emx$

Sketches will vary slightly depending on orientation.

\begin{tikzpicture}[>=latex,x={(-.53cm,-.53cm)},y={(.75cm,0)},z={(0,.75cm)}]
\drawxaxis{-1}{3}{1}{2};
\drawyaxis{-3}{4}{-2}{3};
\drawzaxis{-2}{1}{-1}{-1};
\drawvect{2}{4}{-1}{dotted}{->,thick}{below right}{\vx};
\drawvect{-1}{-3}{-1}{dotted}{->,thick}{below left}{\vy};
\drawvect{1}{1}{-2}{dotted}{->,thick}{below}{$\vx+\vy$};
\drawvect{3}{7}{0}{dotted}{->,thick}{below }{$\vx-\vy$};
\end{tikzpicture}
}