{$\vx = \bmx{c}1\\-1\\2\emx$, $\vy = \bmx{c} 2\\3\\2\emx$}
{$\vx+\vy = \bmx{c}3\\2\\4\emx$, $\vx-\vy = \bmx{c} -1\\-4\\0\emx$

Sketches will vary slightly depending on orientation.

\begin{tikzpicture}[>=latex,x={(-.53cm,-.53cm)},y={(.75cm,0)},z={(0,.75cm)}]
\drawxaxis{-1}{3}{1}{2};
\drawyaxis{-2}{2}{-1}{1};
\drawzaxis{0}{2.5}{1}{2};
\drawvect{2}{3}{4}{dotted}{->,thick}{above right}{\vy};
\drawvect{1}{-1}{2}{dotted}{->,thick}{above left}{\vx};
\drawvect{3}{2}{4}{dotted}{->,thick}{left}{$\vx+\vy$};
\drawvect{-1}{-4}{0}{dotted}{->,thick}{below left}{$\vx-\vy$};
\end{tikzpicture}
}