{$\vx = \bmx{c}0\\1\\1\emx$, $\vy = \bmx{c} 0\\-1\\1\emx$}
{$\vx+\vy = \bmx{c}0\\0\\2\emx$, $\vx-\vy = \bmx{c} 0\\2\\0\emx$

Sketches may vary slightly.

\begin{tikzpicture}[>=latex,x={(-.53cm,-.53cm)},y={(.75cm,0)},z={(0,.75cm)}]
\drawxaxis{0}{2}{1}{1};
\drawyaxis{-1}{2}{1}{1};
\drawzaxis{0}{2}{1}{1};
\drawvect{0}{1}{1}{dotted}{->,thick}{above right}{\vx};
\drawvect{0}{-1}{1}{dotted}{->,thick}{above left}{\vy};
\drawvect{0}{0}{2}{dotted}{->,thick}{right}{$\vx+\vy$};
\drawvect{0}{2}{0}{dotted}{->,thick}{below}{$\vx-\vy$};
\end{tikzpicture}
}